## 分析
```c++
输入  输出
4 3  5
4 5  11
4 7  17
4 9  23
4 11 29
n m  res
res = (4 - 1)m - 4

输入 输出
5 2 3
5 3 7
5 4 11
5 6 19
5 7 23
n m  res
res = (5 - 1)m - 5

输入     输出
111 394 43229
111 395 43339
111 397 43559
111 398 43669
111 400 43889
res = (111 - 1)m - 111

综上，得出公式由n和m凑不出来的最大数为：
res=(n−1)m−n

y总的公式：res = (n - 1)(m - 1) - 1。
```

## 解答
```c++
#include <iostream>
#include <algorithm>

using namespace std;

int main()
{
    int n,m;
    scanf("%d%d", &n, &m);
    
    int ans=n*m-n-m;
    printf("%d",ans);
    
    return 0;
}
```